add an insert that mutates the disk block in place

src/d_find_ins_del/Insert_with_mutation.thy
@@ -1,6 +1,60 @@
 theory Insert_with_mutation
-imports Find "$SRC/c_monad/Insert_state"
+  imports
+"~~/src/HOL/Library/Datatype_Records"
+Monad
 begin
+
+
+lemma FIXME: "P" sorry
+
+(*no termination proof for the following*)
+(*begin iterator*)
+function iter_step :: "('a => 'a option) => 'a => 'a" where
+"iter_step f x = (
+  let r = f x in
+  case r of
+    None => x
+  | Some x => iter_step f x)"
+(*end iterator*)
+apply (force)+ done
+termination iter_step
+ by (force intro:FIXME)
+
+definition rev_apply :: "'a => ('a => 'b) => 'b" (infixl "|>" 100) where
+  "rev_apply x f = f x"
+
+definition failwith :: "String.literal \<Rightarrow> 'b" where
+"failwith x = (STR ''FIXME patch'') |> (% _. undefined)"
+
+
+(* impossible1 marks cases that are impossible; the 1 suffix is needed
+because impossible is reserved (FIXME in OCaml?) *)
+
+definition impossible1 :: "String.literal \<Rightarrow> 'a" where
+  "impossible1 x = failwith x"  
+
+
+(* assert_true always evaluates argument; this is useful for debugging
+OCaml code; FIXME replaced with simple assert in OCaml? *)
+
+definition assert_true :: "bool \<Rightarrow> bool" where
+"assert_true b = (if b then b else failwith (STR ''assert_true''))"
+
+
+(* check_true is patched in OCaml; may evaluate its argument, but can
+be disabled by setting a flag; used during debugging to check various
+conditions; should be disabled in production *)
+
+definition check_true :: "(unit \<Rightarrow> bool) \<Rightarrow> bool" where
+"check_true f = (STR ''FIXME patch'') |> (% _. undefined)"
+
+type_synonym 'k ord = "'k \<Rightarrow> 'k \<Rightarrow> int"
+
+type_synonym 'a s = "'a list"
+
+
+definition key_lt :: "'k ord \<Rightarrow> 'k \<Rightarrow> 'k \<Rightarrow> bool" where
+"key_lt ord k1 k2 = ( ord k1 k2 < 0)"
 
 definition kvs_insert :: "'k ord \<Rightarrow> 'k \<Rightarrow> 'v \<Rightarrow> ('k*'v) s \<Rightarrow> ('k * 'v) s" where "
 kvs_insert k_cmp k v kvs = (
@@ -15,22 +69,55 @@ kvs_insert k_cmp k v kvs = (
   |> (% (kvs,kvs'). (List.rev ((k,v)#kvs))@kvs'))"
 
 
+(* ops types -------------------------------------------- *)
+
+datatype ('k,'v,'r) dnode = 
+  Disk_node "'k list * 'r list" 
+  | Disk_leaf "('k*'v) list"
+
+
 (* read, write, rewrite; rewrite may CoW to produce a new blk ptr *)
+datatype_record ('r,'blk,'t) blk_ops = 
+read :: "('r \<Rightarrow> ('blk,'t) MM)"
+  wrte:: "('blk \<Rightarrow> ('r,'t) MM)"
+  rewrite :: "('r \<Rightarrow> 'blk \<Rightarrow> ('r option,'t) MM)" 
+(*
 type_synonym ('r,'blk,'t) blk_ops = "(
 ('r \<Rightarrow> ('blk,'t) MM) * 
 ('blk \<Rightarrow> ('r,'t) MM) *
 ('r \<Rightarrow> 'blk \<Rightarrow> ('r option,'t) MM))" 
-
+*)
 
 (* blk \<Rightarrow> dnode ; dnode \<Rightarrow> 'blk;  *)
+datatype_record ('blk,'k,'v,'r) marshal_ops = 
+blk2dnode :: "'blk \<Rightarrow> ('k,'v,'r) dnode"
+dnode2blk :: "('k,'v,'r) dnode \<Rightarrow> 'blk"
+
+(*
 type_synonym ('blk,'k,'v,'r) marshal_ops = "(
 ('blk \<Rightarrow> ('k,'v,'r) dnode) * 
 (('k,'v,'r) dnode \<Rightarrow> 'blk))"
+*)
 
 (* alloc; free *) 
+datatype_record ('r,'t) alloc_ops = 
+alloc :: "unit \<Rightarrow> ('r,'t) MM"
+free :: "'r s \<Rightarrow> (unit,'t) MM"
+
+(*
 type_synonym ('r,'t) alloc_ops = "(
 (unit \<Rightarrow> ('r,'t) MM) *
 ('r s \<Rightarrow> (unit,'t) MM))"
+*)
+
+
+
+datatype_record constants = 
+  min_leaf_size :: nat
+  max_leaf_size :: nat
+  min_node_keys :: nat
+  max_node_keys :: nat
+
 
 
 datatype ('a,'b,'c) stk_frame = Frm "'a * 'b * 'c"
@@ -46,6 +133,9 @@ type_synonym ('k,'r) frame = "( ('r list * 'k list), 'r, ('k list * 'r list)) st
 type_synonym ('k,'r) stk = "('k,'r) frame list"
 
 
+(* find ------------------------------- *)
+
+
 datatype ('k,'v,'r) find_state = 
   F_down "'r * 'k * 'r * ('k,'r) stk"  (* root, search key, current pointer, stack *) 
   | F_finished "'r * 'k * 'r * ('k*'v)s * ('k,'r)stk"
@@ -56,11 +146,14 @@ definition dest_F_finished :: "('k,'v,'r)find_state \<Rightarrow> ('r*'k*'r*('k*
   F_down _ \<Rightarrow> None
   | F_finished (r0,k,r,kvs,stk) \<Rightarrow> Some(r0,k,r,kvs,stk) )"
 
+definition make_initial_find_state :: "'k \<Rightarrow> 'r \<Rightarrow> ('k,'v,'r) find_state" where "
+make_initial_find_state k r = F_down (r,k,r,[])"
+
 (* walk through ks and rs to find the point where ki \<le> k < k(i+1); |ks|+1=|rs|;
 or: find first point where k < ki
  *)
-definition find_split_node :: "'k ord \<Rightarrow> 'k \<Rightarrow> 'k s \<Rightarrow> 'r s \<Rightarrow> ('k,'r)frame * 'r" where
-"find_split_node k_cmp k ks rs = (
+definition make_frame :: "'k ord \<Rightarrow> 'k \<Rightarrow> 'k s \<Rightarrow> 'r s \<Rightarrow> ('k,'r)frame * 'r" where
+"make_frame k_cmp k ks rs = (
   iter_step (% ((rs,ks),(ks',rs')).
     case ks' of 
     [] \<Rightarrow> None
@@ -76,9 +169,6 @@ definition find_split_node :: "'k ord \<Rightarrow> 'k \<Rightarrow> 'k s \<Righ
      (Frm((rs,ks),r',(ks',List.tl rs')),  r')))"
 
 
-(* Some(Frm((ks,rs),List.hd rs',([],[]))) *)
-
-(* find ------------------------------- *)
 
 definition find_step :: "
 constants \<Rightarrow> 
@@ -87,18 +177,19 @@ constants \<Rightarrow>
 ('blk,'k,'v,'r) marshal_ops \<Rightarrow> 
 ('r,'t) alloc_ops \<Rightarrow>  
 ('k,'v,'r) find_state \<Rightarrow> (('k,'v,'r) find_state,'t) MM" where
-"find_step cs k_cmp blk_ops marshal_ops alloc_ops fs = (
-  let (read,write,rewrite) = blk_ops in
-  let (blk2frm,_) = marshal_ops in
+"find_step cs k_cmp blk_ops marshal_ops alloc_ops = (
+  let read = blk_ops|>read in
+  let blk2dnode = marshal_ops|>blk2dnode in
+  (% fs. 
   case fs of 
   F_finished _ \<Rightarrow> return fs \<comment> \<open> stutter; or fail? \<close>
   | F_down(r0,k,r,stk) \<Rightarrow> (
-    read r |>fmap blk2frm |>fmap (% f. 
+    read r |>fmap blk2dnode |>fmap (% f. 
     case f of 
     Disk_node (ks,rs) \<Rightarrow> (
-      let (frm,r) = find_split_node k_cmp k ks rs in      
+      let (frm,r) = make_frame k_cmp k ks rs in      
       F_down(r0,k,r,frm#stk))
-    | Disk_leaf kvs \<Rightarrow> F_finished(r0,k,r,kvs,stk))))"
+    | Disk_leaf kvs \<Rightarrow> F_finished(r0,k,r,kvs,stk)))))"
 
 
 
@@ -118,6 +209,7 @@ datatype (dead 'k,dead 'v,dead 'r) insert_state =
   I_down "('k,'v,'r) d"
   | I_up "('k,'v,'r) u"
   | I_finished 'r
+  | I_finished_with_mutate
 
 definition step_down :: "
 constants \<Rightarrow> 
@@ -126,9 +218,25 @@ constants \<Rightarrow>
 ('blk,'k,'v,'r) marshal_ops \<Rightarrow> 
 ('r,'t) alloc_ops \<Rightarrow> 
 ('k,'v,'r) d \<Rightarrow> (('k,'v,'r) d,'t) MM" where
-"step_down cs k_cmp blk_ops marshal_ops alloc_ops d = (
+"step_down cs k_cmp blk_ops marshal_ops alloc_ops = (
+  let find_step =  find_step cs k_cmp blk_ops marshal_ops alloc_ops in
+  (% d.
   let (fs,v) = d in
-  find_step cs k_cmp blk_ops marshal_ops alloc_ops fs |> fmap (% d'. (d',v)) )"
+  find_step fs |> fmap (% d'. (d',v)) ))"
+
+definition split_leaf :: "constants \<Rightarrow> ('k*'v) s \<Rightarrow> ('k*'v)s * 'k * ('k*'v) s" where "
+split_leaf cs kvs = (
+  let _ = assert_true True in
+  iter_step (% (kvs,kvs').
+    case List.length kvs' \<le> cs|>min_leaf_size of
+    True \<Rightarrow> None
+    | False \<Rightarrow> (
+      case kvs' of 
+      [] \<Rightarrow> impossible1 (STR ''split_leaf'')
+      | (k,v)#kvs' \<Rightarrow> Some((k,v)#kvs,kvs')))
+    ([],kvs)
+  |> (% (kvs,kvs'). (List.rev kvs,List.hd kvs'|>fst, kvs')))
+"
 
 definition step_bottom :: "
 constants \<Rightarrow> 
@@ -138,9 +246,9 @@ constants \<Rightarrow>
 ('r,'t) alloc_ops \<Rightarrow> 
 ('k,'v,'r) d \<Rightarrow> (('k,'v,'r) u + unit,'t) MM" where
 "step_bottom cs k_cmp blk_ops marshal_ops alloc_ops d = (
-  let (read,write,rewrite) = blk_ops in
-  let (_,dnode2blk) = marshal_ops in
-  let (alloc,free) = alloc_ops in
+  let (write,rewrite) = (blk_ops|>wrte,blk_ops|>rewrite) in
+  let dnode2blk = marshal_ops|>dnode2blk in
+  let alloc = alloc_ops|>alloc in
   let (fs,v) = d in
   case dest_F_finished fs of 
   None \<Rightarrow> impossible1 (STR ''insert, step_bottom'')
@@ -171,6 +279,31 @@ definition unsplit_node :: "('r s * 'k s) * ('r s * 'k s) * ('k s * 'r s) \<Righ
   let ((rs1,ks1),(rs2,ks2),(ks3,rs3)) = x in
   ( (List.rev ks1)@ks2@ks3, (List.rev rs1)@rs2@rs3) )"
 
+(* NOTE for both split_node and split_leaf, we may know the order is dense, and all keys have values; in which case we can split
+with a full left leaf/node *)
+definition split_node :: 
+  "constants \<Rightarrow> ('k list * 'a list) \<Rightarrow> ('k list * 'a list) * 'k * ('k list * 'a list)" 
+where
+"split_node cs n = (
+  let (ks,rs) = n in
+  let l = List.length ks  div 2 in
+  let l = max (cs|>min_node_keys) l in
+  iter_step (% (ks,rs,ks',rs').
+    case (ks',rs') of 
+    (k'#ks',r'#rs') \<Rightarrow> (
+      case List.length ks < l of
+      True \<Rightarrow> Some(k'#ks,r'#rs,ks',rs')
+      | False \<Rightarrow> None)
+    | _ \<Rightarrow> (impossible1 (STR ''split_node'')))
+    ([],[],ks,rs)
+  |> (% (ks,rs,ks',rs').
+    case (ks',rs') of
+    (k'#ks',r'#rs') \<Rightarrow> (
+      (List.rev ks,List.rev(r'#rs)),
+      k',
+      (ks',rs'))))"
+
+
 definition step_up :: "
 constants \<Rightarrow> 
 'k ord \<Rightarrow> 
@@ -179,9 +312,9 @@ constants \<Rightarrow>
 ('r,'t) alloc_ops \<Rightarrow> 
 ('k,'v,'r) u \<Rightarrow> (('k,'v,'r) u,'t) MM" where
 "step_up  cs k_cmp blk_ops marshal_ops alloc_ops u = (
-  let (read,write,rewrite) = blk_ops in
-  let (_,dnode2blk) = marshal_ops in
-  let (alloc,free) = alloc_ops in
+  let (write,rewrite) = (blk_ops|>wrte,blk_ops|>rewrite) in
+  let dnode2blk = marshal_ops|>dnode2blk in
+  let alloc = alloc_ops|>alloc in
   let (fo,stk) = u in
   case stk of 
   [] \<Rightarrow> impossible1 (STR ''insert, step_up'') 
@@ -208,15 +341,31 @@ constants \<Rightarrow>
         write blk |> bind (% r2.
         return (I2(r1,k,r2),stk')))) )))))"
 
-(*
-definition insert_step :: "'k ps1 \<Rightarrow> ('k,'v,'r,'t) store_ops \<Rightarrow> ('k,'v,'r) ist \<Rightarrow> (('k,'v,'r) ist,'t) MM" where
-"insert_step ps1 store_ops s = (
+
+definition insert_step :: "
+constants \<Rightarrow> 
+'k ord \<Rightarrow> 
+('r,'blk,'t) blk_ops \<Rightarrow>
+('blk,'k,'v,'r) marshal_ops \<Rightarrow> 
+('r,'t) alloc_ops \<Rightarrow> 
+('k,'v,'r) insert_state \<Rightarrow> (('k,'v,'r) insert_state,'t) MM" where
+"insert_step cs k_cmp  blk_ops marshal_ops alloc_ops = (
+  let step_down = step_down cs k_cmp  blk_ops marshal_ops alloc_ops in
+  let step_bottom = step_bottom cs k_cmp  blk_ops marshal_ops alloc_ops in
+  let step_up = step_up  cs k_cmp blk_ops marshal_ops alloc_ops in
+  let write = blk_ops|>wrte in
+  let dnode2blk = marshal_ops|>dnode2blk in
+  let alloc = alloc_ops|>alloc in
+  (% s.
   case s of 
   I_down d \<Rightarrow> (
     let (fs,v) = d in
-    case (dest_f_finished fs) of 
-    None \<Rightarrow> (step_down ps1 store_ops d |> fmap (% d. I_down d))
-    | Some _ \<Rightarrow> step_bottom ps1 store_ops d |> fmap (% u. I_up u))
+    case dest_F_finished fs of 
+    None \<Rightarrow> (step_down d |> fmap (% d. I_down d))
+    | Some _ \<Rightarrow> step_bottom d |> bind (% bot.
+      case bot of 
+      Inr () \<Rightarrow> return I_finished_with_mutate
+      | Inl u \<Rightarrow> return (I_up u)))
   | I_up u \<Rightarrow> (
     let (fo,stk) = u in
     case stk of
@@ -224,10 +373,26 @@ definition insert_step :: "'k ps1 \<Rightarrow> ('k,'v,'r,'t) store_ops \<Righta
       case fo of 
       I1 r \<Rightarrow> return (I_finished r)
       | I2(r1,k,r2) \<Rightarrow> (
-        (mk_Disk_node([k],[r1,r2]) |> (store_ops|>store_alloc) |> fmap (% r. I_finished r))))
-    | _ \<Rightarrow> (step_up ps1 store_ops u |> fmap (% u. I_up u)))
-  | I_finished f \<Rightarrow> (return s)  \<comment> \<open> stutter \<close> )"
-*)
+        (Disk_node([k],[r1,r2]) |> dnode2blk |> (% blk.
+        write blk |> bind (% r.
+        return (I_finished r))))))
+    | _ \<Rightarrow> (step_up u |> fmap (% u. I_up u)))
+  | I_finished _ \<Rightarrow> (return s)  \<comment> \<open> stutter \<close> 
+  | I_finished_with_mutate \<Rightarrow> (return s)))"
 
 
+export_code  
+"Code_Numeral.int_of_integer"
+fmap
+Disk_node
+make_constants
+make_alloc_ops
+make_blk_ops
+make_marshal_ops
+make_initial_find_state
+I1
+I_down
+insert_step
+
+in OCaml file "/tmp/insert_with_mutation.ml"
 end
