src/d_find_ins_del/Monad.thy
@@ -1,0 +1,20 @@
+theory Monad
+imports Main
+begin
+
+
+(* abstract version; NOTE obviously can't be exported *)
+(* NOTE undefined is accepted by the code generator and allows these abstract defns to be exported *)
+typedecl ('a,'b) MM
+
+definition fmap :: "('a \<Rightarrow> 'b) \<Rightarrow> ('a,'t) MM \<Rightarrow> ('b,'t) MM" where
+"fmap x y = undefined"
+
+definition bind :: "('a \<Rightarrow> ('b,'t) MM) \<Rightarrow> ('a,'t) MM \<Rightarrow> ('b,'t) MM" where
+"bind b a = undefined"
+  
+definition return :: "'a \<Rightarrow> ('a,'t) MM" where
+"return x = undefined"
+
+
+end
